theories/Algebra/Homological/Biproducts.v
@@ -1,0 +1,1017 @@
+Require Import Basics.Overture Basics.Decidable Basics.Tactics Basics.Trunc.
+Require Import WildCat.Core WildCat.Products WildCat.Coproducts WildCat.Equiv.
+Require Import WildCat.PointedCat WildCat.Bifunctor WildCat.NatTrans WildCat.Prod.
+Require Import WildCat.Monoidal.
+Require Import Types.Bool Types.Forall.
+Require Import Algebra.AbGroups.AbelianGroup.
+Require Import WildCat.Square.
+
+(** * Categories with biproducts *)
+
+(** ** Biproducts *)
+
+Class Biproduct (I : Type) `{DecidablePaths I} {A : Type}
+  `{HasEquivs A, !IsPointedCat A} {x : I -> A}
+  := Build_Biproduct' {
+  biproduct_product :: Product I x;
+  biproduct_coproduct :: Coproduct I x;
+  catie_cat_coprod_prod_incl :: CatIsEquiv (cat_coprod_prod_incl x);
+}.
+
+Arguments Biproduct I {_ A _ _ _ _ _ _} x.
+
+Section Biproducts.
+  Context {I : Type} {A : Type} (x : I -> A) `{Biproduct I A x}.
+  
+  Definition cate_coprod_prod : cat_coprod I x $<~> cat_prod I x
+    := Build_CatEquiv (cat_coprod_prod_incl x).
+
+  Definition cat_biprod : A
+    := cat_prod I x.
+
+  Definition cat_biprod_pr : forall (i : I), cat_biprod $-> x i
+    := cat_pr.
+
+  Definition cat_biprod_corec {z : A}
+    : (forall i, z $-> x i) -> z $-> cat_biprod
+    := cat_prod_corec I.
+
+  Definition cat_biprod_corec_beta {z : A} (f : forall i, z $-> x i)
+    : forall i, cat_biprod_pr i $o cat_biprod_corec f $== f i
+    := cat_prod_beta I f.
+
+  Definition cat_biprod_corec_eta {z : A} (f : z $-> cat_biprod)
+    : cat_biprod_corec (fun i => cat_biprod_pr i $o f) $== f
+    := cat_prod_eta I f.
+  
+  Definition cat_biprod_corec_eta' {z : A} {f f' : forall i, z $-> x i}
+    : (forall i, f i $== f' i) -> cat_biprod_corec f $== cat_biprod_corec f'
+    := cat_prod_corec_eta I.
+  
+  Definition cat_biprod_pr_eta {z : A} {f f' : z $-> cat_biprod}
+    : (forall i, cat_biprod_pr i $o f $== cat_biprod_pr i $o f') -> f $== f'
+    := cat_prod_pr_eta I.
+
+  Definition cat_biprod_in : forall (i : I), x i $-> cat_biprod
+    := fun i => cate_coprod_prod $o cat_in i.
+
+  Definition cat_biprod_rec {z : A}
+    : (forall i, x i $-> z) -> cat_biprod $-> z
+    := fun f => cat_coprod_rec I f $o cate_coprod_prod^-1$. 
+
+  Definition cat_biprod_rec_beta {z : A} (f : forall i, x i $-> z)
+    : forall i, cat_biprod_rec f $o cat_biprod_in i $== f i.
+  Proof.
+    intros i.
+    unfold cat_biprod_rec, cat_biprod_in.
+    refine (_ $@ cat_coprod_beta I f i).
+    nrefine (cat_assoc _ _ _ $@ (_ $@L _)).
+    apply compose_V_hh.
+  Defined.
+
+  Definition cat_biprod_rec_eta {z : A} (f : cat_biprod $-> z)
+    : cat_biprod_rec (fun i => f $o cat_biprod_in i) $== f.
+  Proof.
+    unfold cat_biprod_rec.
+    apply cate_moveR_eV.
+    apply cat_coprod_in_eta.
+    intros i.
+    refine (cat_coprod_beta I _ i $@ _^$).
+    apply cat_assoc.
+  Defined.
+
+  Definition cat_biprod_rec_eta' {z : A} {f f' : forall i, x i $-> z}
+    : (forall i, f i $== f' i) -> cat_biprod_rec f $== cat_biprod_rec f'.
+  Proof.
+    intros p.
+    unfold cat_biprod_rec.
+    exact (cat_coprod_rec_eta I p $@R _).
+  Defined.
+
+  Definition cat_biprod_in_eta {z : A} {f f' : cat_biprod $-> z}
+    : (forall i, f $o cat_biprod_in i $== f' $o cat_biprod_in i) -> f $== f'.
+  Proof.
+    intros p.
+    apply (cate_epic_equiv cate_coprod_prod).
+    apply cat_coprod_in_eta.
+    intros i.
+    exact (cat_assoc _ _ _ $@ p i $@ (cat_assoc _ _ _)^$).
+  Defined.
+
+End Biproducts.
+
+Arguments cat_biprod I {A} x {_ _ _ _ _ _ _ _}.
+Arguments cat_biprod_pr {I A x _ _ _ _ _ _ _ _} i.
+Arguments cat_biprod_in {I A x _ _ _ _ _ _ _ _} i.
+Arguments cate_coprod_prod {I A} x {_ _ _ _ _ _ _ _}.
+
+(** An inclusion followed by a projection of the same index is the identity. *)
+Definition cat_biprod_pr_in (I : Type) {A : Type} (x : I -> A)
+  `{Biproduct I A x} (i : I)
+  : cat_biprod_pr i $o cat_biprod_in i $== Id _.
+Proof.
+  unfold cat_biprod_pr, cat_biprod_in.
+  refine ((_ $@L _) $@ _).
+  { refine ((cate_buildequiv_fun _ $@R _) $@ _).
+    apply cat_coprod_beta. }
+  refine (cat_prod_beta _ _ _ $@ _).
+  destruct (dec_paths i i); simpl.
+  - (** We cannot eliminate [p : i = i] with path induction, but we do have decidable equality, hence by Hedberg's theorem we must be in a hset and we can replace this with the identity. *)
+    assert (r : (idpath = p)) by apply path_ishprop.
+    by destruct r.
+  - contradiction n.
+    reflexivity.
+Defined.
+
+(** An inclusion followed by a projection of a different index is zero. *)
+Definition cat_biprod_pr_in_ne (I : Type) {A : Type} (x : I -> A)
+  `{Biproduct I A x} {i j : I} (p : i <> j)
+  : cat_biprod_pr j $o cat_biprod_in i $== zero_morphism.
+Proof.
+  unfold cat_biprod_pr, cat_biprod_in.
+  refine ((_ $@L _) $@ _).
+  { refine ((cate_buildequiv_fun _ $@R _) $@ _).
+    apply cat_coprod_beta. }
+  refine (cat_prod_beta _ _ _ $@ _).
+  destruct (dec_paths i j); simpl.
+  - contradiction p.
+  - reflexivity.
+Defined.
+
+Definition cat_biprod_diag I {A} (x : A) `{Biproduct I A (fun _ => x)}
+  : x $-> cat_biprod I (fun _ => x)
+  := cat_prod_diag x.
+
+Definition cat_biprod_codiag I {A} (x : A) `{Biproduct I A (fun _ => x)}
+  : cat_biprod I (fun _ => x) $-> x
+  := cat_coprod_fold x $o (cate_coprod_prod (fun _ => x))^-1$.
+
+(** Compatability of [cat_biprod_rec] and [cat_biprod_corec]. *)
+Definition cat_biprod_corec_rec I `{DecidablePaths I} {A : Type}
+  `{HasEquivs A, !IsPointedCat A} {x y : I -> A}
+  `{!Biproduct I x, !Biproduct I y}
+  (f : forall i, x i $-> y i)
+  : cat_biprod_corec y (fun i => f i $o cat_biprod_pr i)
+    $== cat_biprod_rec x (fun i => cat_biprod_in i $o f i).
+Proof.
+  apply cat_biprod_pr_eta.
+  intros i.
+  refine (cat_biprod_corec_beta _ _ i $@ _).
+  apply cat_biprod_in_eta.
+  intros j.
+  refine (_ $@ (_ $@L (cat_biprod_rec_beta _ _ _)^$) $@ (cat_assoc _ _ _)^$).
+  refine (cat_assoc _ _ _ $@ _ $@ cat_assoc _ _ _).
+  destruct (dec_paths j i) as [p | np].
+  - destruct p.
+    refine ((_ $@L _) $@ cat_idr _ $@ (cat_idl _)^$ $@ (_^$ $@R _)).
+    1,2: apply cat_biprod_pr_in.
+  - refine ((_ $@L _) $@ cat_zero_r _ $@ (cat_zero_l _)^$ $@ (_^$ $@R _)).
+    1,2: apply cat_biprod_pr_in_ne, np.
+Defined.
+
+(** *** Existence of biproducts *)
+ 
+Class HasBiproducts (I A : Type)
+  `{DecidablePaths I, HasEquivs A, !IsPointedCat A}
+  := has_biproducts :: forall (x : I -> A), Biproduct I x.
+
+(** *** Binary biproducts *)
+
+Class BinaryBiproduct {A : Type} `{HasEquivs A, !IsPointedCat A} (x y : A)
+  := binary_biproduct :: Biproduct Bool (fun b => if b then x else y).
+  
+Class HasBinaryBiproducts (A : Type) `{HasEquivs A, !IsPointedCat A}
+  := has_binary_biproducts :: forall (x y : A), BinaryBiproduct x y.
+
+Global Instance hasbinarybiproducts_hasbiproductsbool {A : Type}
+  `{HasEquivs A, !IsPointedCat A, !HasBiproducts Bool A}
+  : HasBinaryBiproducts A
+  := fun x y => has_biproducts (fun b : Bool => if b then x else y).
+
+Global Instance hasbinaryproducts_hasbinarybiproducts {A : Type}
+  `{H : HasBinaryBiproducts A}
+  : HasBinaryProducts A.
+Proof.
+  intros x y.
+  apply biproduct_product.
+Defined.
+
+Global Instance hasbinarycoproducts_hasbinarybiproducts {A : Type}
+  `{H : HasBinaryBiproducts A}
+  : HasBinaryCoproducts A.
+Proof.
+  intros x y.
+  nrapply biproduct_coproduct.
+  apply H.
+Defined.
+
+Section BinaryBiproducts.
+
+  Context {A : Type} `{HasEquivs A, !IsPointedCat A} {x y : A}
+    `{!BinaryBiproduct x y}.
+
+  Definition cat_binbiprod : A
+    := cat_biprod Bool (fun b => if b then x else y).
+  
+  Definition cat_binbiprod_pr1 : cat_binbiprod $-> x := cat_biprod_pr true.
+  Definition cat_binbiprod_pr2 : cat_binbiprod $-> y := cat_biprod_pr false.
+  
+  Definition cat_binbiprod_corec {z : A} (f : z $-> x) (g : z $-> y)
+    : z $-> cat_binbiprod.
+  Proof.
+    apply cat_biprod_corec.
+    intros [|].
+    - exact f.
+    - exact g.
+  Defined.
+
+  Definition cat_binbiprod_corec_beta_pr1 {z : A} (f : z $-> x) (g : z $-> y)
+    : cat_binbiprod_pr1 $o cat_binbiprod_corec f g $== f
+    := cat_biprod_corec_beta _ _ true.
+
+  Definition cat_binbiprod_corec_beta_pr2 {z : A} (f : z $-> x) (g : z $-> y)
+    : cat_binbiprod_pr2 $o cat_binbiprod_corec f g $== g
+    := cat_biprod_corec_beta _ _ false.
+
+  Definition cat_binbiprod_corec_eta {z : A} (f : z $-> cat_binbiprod)
+    : cat_binbiprod_corec (cat_binbiprod_pr1 $o f) (cat_binbiprod_pr2 $o f)
+      $== f.
+  Proof.
+    apply cat_biprod_pr_eta.
+    intros [|].
+    - exact (cat_binbiprod_corec_beta_pr1 _ _).
+    - exact (cat_binbiprod_corec_beta_pr2 _ _).
+  Defined.
+
+  Definition cat_binbiprod_corec_eta' {z : A} {f f' : z $-> x} {g g' : z $-> y}
+    : f $== f' -> g $== g'
+      -> cat_binbiprod_corec f g $== cat_binbiprod_corec f' g'.
+  Proof.
+    intros p q.
+    apply cat_biprod_corec_eta'.
+    intros [|].
+    - exact p.
+    - exact q.
+  Defined.
+
+  Definition cat_binbiprod_pr_eta {z : A} {f f' : z $-> cat_binbiprod}
+     : cat_binbiprod_pr1 $o f $== cat_binbiprod_pr1 $o f'
+      -> cat_binbiprod_pr2 $o f $== cat_binbiprod_pr2 $o f'
+      -> f $== f'.
+  Proof.
+    intros p q.
+    apply cat_biprod_pr_eta.
+    intros [|].
+    - exact p.
+    - exact q.
+  Defined.
+
+  Definition cat_binbiprod_inl : x $-> cat_binbiprod := cat_biprod_in true.
+  Definition cat_binbiprod_inr : y $-> cat_binbiprod := cat_biprod_in false.
+
+  Definition cat_binbiprod_rec {z : A} (f : x $-> z) (g : y $-> z)
+    : cat_binbiprod $-> z.
+  Proof.
+    apply cat_biprod_rec.
+    intros [|].
+    - exact f.
+    - exact g.
+  Defined.
+
+  Definition cat_binbiprod_rec_beta_inl {z : A} (f : x $-> z) (g : y $-> z)
+    : cat_binbiprod_rec f g $o cat_binbiprod_inl $== f
+    := cat_biprod_rec_beta _ _ true.
+  
+  Definition cat_binbiprod_rec_beta_inr {z : A} (f : x $-> z) (g : y $-> z)
+    : cat_binbiprod_rec f g $o cat_binbiprod_inr $== g
+    := cat_biprod_rec_beta _ _ false.
+
+  Definition cat_binbiprod_rec_eta {z : A} (f : cat_binbiprod $-> z)
+    : cat_binbiprod_rec (f $o cat_binbiprod_inl) (f $o cat_binbiprod_inr) $== f.
+  Proof.
+    apply cat_biprod_in_eta.
+    intros [|].
+    - exact (cat_binbiprod_rec_beta_inl _ _).
+    - exact (cat_binbiprod_rec_beta_inr _ _).
+  Defined.
+
+  Definition cat_binbiprod_rec_eta' {z : A} {f f' : x $-> z} {g g' : y $-> z}
+    : f $== f' -> g $== g'
+      -> cat_binbiprod_rec f g $== cat_binbiprod_rec f' g'.
+  Proof.
+    intros p q.
+    apply cat_biprod_rec_eta'.
+    intros [|].
+    - exact p.
+    - exact q.
+  Defined.
+
+  Definition cat_binbiprod_in_eta {z : A} {f f' : cat_binbiprod $-> z}
+    : f $o cat_binbiprod_inl $== f' $o cat_binbiprod_inl
+      -> f $o cat_binbiprod_inr $== f' $o cat_binbiprod_inr
+      -> f $== f'.
+  Proof.
+    intros p q.
+    apply cat_biprod_in_eta.
+    intros [|].
+    - exact p.
+    - exact q.
+  Defined.
+
+  Definition cat_binbiprod_pr1_inl
+    : cat_binbiprod_pr1 $o cat_binbiprod_inl $== Id _
+    := cat_biprod_pr_in Bool _ true.
+
+  Definition cat_binbiprod_pr2_inr
+    : cat_binbiprod_pr2 $o cat_binbiprod_inr $== Id _
+    := cat_biprod_pr_in Bool _ false.
+
+  Definition cat_binbiprod_pr2_inl
+    : cat_binbiprod_pr2 $o cat_binbiprod_inl $== zero_morphism.
+  Proof.
+    snrapply (cat_biprod_pr_in_ne Bool _ (i := true) (j := false)).
+    apply (not_fixed_negb false).
+  Defined.
+  
+  Definition cat_binbiprod_pr1_inr
+    : cat_binbiprod_pr1 $o cat_binbiprod_inr $== zero_morphism.
+  Proof.
+    snrapply (cat_biprod_pr_in_ne Bool _ (i := false) (j := true)).
+    apply (not_fixed_negb true).
+  Defined.
+
+End BinaryBiproducts.
+
+Arguments cat_binbiprod {A _ _ _ _ _ _} x y {_}.
+
+(** Annoyingly this doesn't follow directly from the general diagonal since [fun b => if b then x else x] is not definitionally equal to [fun _ => x]. *)
+Definition cat_binbiprod_diag {A : Type}
+  `{HasEquivs A, !IsPointedCat A} (x : A) `{!BinaryBiproduct x x}
+  : x $-> cat_binbiprod x x.
+Proof.
+  snrapply cat_binbiprod_corec; exact (Id _).
+Defined.
+
+Definition cat_binbiprod_codiag {A : Type}
+  `{HasEquivs A, !IsPointedCat A} (x : A) `{!BinaryBiproduct x x}
+  : cat_binbiprod x x $-> x.
+Proof.
+  snrapply cat_binbiprod_rec; exact (Id _).
+Defined.
+
+(** Compatability of [cat_binprod_rec] and [cat_binprod_corec]. *)
+Definition cat_binbiprod_corec_rec {A : Type}
+  `{HasEquivs A, !IsPointedCat A} {w x y z : A}
+  `{!BinaryBiproduct w x, !BinaryBiproduct y z}
+  (f : w $-> y) (g : x $-> z)
+  : cat_binbiprod_corec (f $o cat_binbiprod_pr1) (g $o cat_binbiprod_pr2)
+    $== cat_binbiprod_rec (cat_binbiprod_inl $o f) (cat_binbiprod_inr $o g).
+Proof.
+  unfold cat_binbiprod_corec, cat_binbiprod_rec.
+  nrefine (_ $@ _ $@ _).
+  2: snrapply cat_biprod_corec_rec; by intros [|].
+  1: snrapply cat_biprod_corec_eta'; by intros [|].
+  snrapply cat_biprod_rec_eta'; by intros [|].
+Defined.
+
+(** *** Binary biproduct bifunctor *)
+
+Global Instance is0bifunctor_cat_binbiprod {A : Type}
+  `{HasBinaryBiproducts A}
+  : Is0Bifunctor (fun x y : A => cat_binbiprod x y)
+  := is0bifunctor_cat_binprod.
+
+Global Instance is1bifunctor_cat_binbiprod {A : Type}
+  `{HasBinaryBiproducts A}
+  : Is1Bifunctor (fun x y : A => cat_binbiprod x y)
+  := is1bifunctor_cat_binprod.
+
+(** Binary biproducts are functorial in each argument. *)
+Global Instance is0functor_cat_binbiprod_l {A : Type}
+  `{HasBinaryBiproducts A} (y : A)
+  : Is0Functor (fun x => cat_binbiprod x y)
+  := bifunctor_is0functor10 y.
+
+Global Instance is1functor_cat_binbiprod_l {A : Type}
+  `{HasBinaryBiproducts A} (y : A)
+  : Is1Functor (fun x => cat_binbiprod x y)
+  := bifunctor_is1functor10 y.
+
+Global Instance is0functor_cat_binbiprod_r {A : Type}
+  `{HasBinaryBiproducts A} (x : A)
+  : Is0Functor (fun y => cat_binbiprod x y)
+  := bifunctor_is0functor01 x.
+
+Global Instance is1functor_cat_binbiprod_r {A : Type}
+  `{HasBinaryBiproducts A} (x : A)
+  : Is1Functor (fun y => cat_binbiprod x y)
+  := bifunctor_is1functor01 x.
+
+(** *** Symmetry *)
+
+Section Symmetry.
+  Context {A : Type} `{HasBinaryBiproducts A}.
+
+  Definition cat_binbiprod_swap (x y : A)
+    : cat_binbiprod x y $-> cat_binbiprod y x
+    := cat_binbiprod_corec cat_binbiprod_pr2 cat_binbiprod_pr1.
+
+  Lemma cat_binbiprod_swap_swap (x y : A)
+    : cat_binbiprod_swap x y $o cat_binbiprod_swap y x $== Id _.
+  Proof.
+    rapply cat_binprod_swap_cat_binprod_swap.
+  Defined.
+
+  Local Instance symmetricbraiding_cat_binbiprod
+    : SymmetricBraiding (fun x y => cat_binbiprod x y). 
+  Proof.
+    rapply symmetricbraiding_binprod.
+  Defined.
+
+  Lemma cat_binbiprod_swap_inl (x y : A)
+    : cat_binbiprod_swap x y $o cat_binbiprod_inl
+      $== cat_binbiprod_inr.
+  Proof.
+    apply cat_binbiprod_pr_eta.
+    - refine ((cat_assoc _ _ _)^$ $@ _).
+      refine ((_ $@R _) $@ _).
+      1: apply cat_binbiprod_corec_beta_pr1.
+      refine (_ $@ _^$).
+      1: apply cat_binbiprod_pr2_inl.
+      apply cat_binbiprod_pr1_inr.
+    - refine ((cat_assoc _ _ _)^$ $@ _).
+      refine ((_ $@R _) $@ _).
+      1: apply cat_binbiprod_corec_beta_pr2.
+      refine (_ $@ _^$).
+      1: apply cat_binbiprod_pr1_inl.
+      apply cat_binbiprod_pr2_inr.
+  Defined.
+  
+  Lemma cat_binbiprod_swap_inr (x y : A)
+    : cat_binbiprod_swap x y $o cat_binbiprod_inr
+      $== cat_binbiprod_inl.
+  Proof.
+    apply cat_binbiprod_pr_eta.
+    - refine ((cat_assoc _ _ _)^$ $@ _).
+      refine ((_ $@R _) $@ _).
+      1: apply cat_binbiprod_corec_beta_pr1.
+      refine (_ $@ _^$).
+      1: apply cat_binbiprod_pr2_inr.
+      apply cat_binbiprod_pr1_inl.
+    - refine ((cat_assoc _ _ _)^$ $@ _).
+      refine ((_ $@R _) $@ _).
+      1: apply cat_binbiprod_corec_beta_pr2.
+      refine (_ $@ _^$).
+      1: apply cat_binbiprod_pr1_inr.
+      apply cat_binbiprod_pr2_inl.
+  Defined.
+    
+  (** The swap map preserves the diagonal. *)
+  Lemma cat_binbiprod_swap_diag (x : A)
+    : cat_binbiprod_swap x x $o cat_binbiprod_diag x $== cat_binbiprod_diag x.
+  Proof.
+    apply cat_binbiprod_pr_eta.
+    - refine ((cat_assoc _ _ _)^$ $@ (_ $@R _) $@ _).
+      1: apply cat_binbiprod_corec_beta_pr1.
+      refine (cat_binbiprod_corec_beta_pr2 _ _ $@ _^$).
+      apply cat_binbiprod_corec_beta_pr1.
+    - refine ((cat_assoc _ _ _)^$ $@ (_ $@R _) $@ _).
+      1: apply cat_binbiprod_corec_beta_pr2.
+      refine (cat_binbiprod_corec_beta_pr1 _ _ $@ _^$).
+      apply cat_binbiprod_corec_beta_pr2.
+  Defined.
+  
+  (** The swap map preserves the codiagonal. TODO: proof can probably be shorter. *)
+  Lemma cat_binbiprod_swap_codiag (x : A)
+    : cat_binbiprod_codiag x $o cat_binbiprod_swap x x $== cat_binbiprod_codiag x.
+  Proof.
+    apply cat_binbiprod_in_eta.
+    - refine (_ $@ (cat_binbiprod_rec_beta_inl _ _)^$).
+      refine (cat_assoc _ _ _ $@ (_ $@L _) $@ _).
+      + apply cat_binbiprod_pr_eta.
+        * refine ((cat_assoc _ _ _)^$ $@ (_ $@R _) $@ _).
+          1: apply cat_binbiprod_corec_beta_pr1.
+          refine (_ $@ _^$).
+          1: apply cat_binbiprod_pr2_inl.
+          apply cat_binbiprod_pr1_inr.
+        * refine ((cat_assoc _ _ _)^$ $@ (_ $@R _) $@ _).
+          1: apply cat_binbiprod_corec_beta_pr2.
+          refine (_ $@ _^$).
+          1: apply cat_binbiprod_pr1_inl.
+          apply cat_binbiprod_pr2_inr.
+      + apply cat_binbiprod_rec_beta_inr.
+    - refine (_ $@ (cat_binbiprod_rec_beta_inr _ _)^$).
+      refine (cat_assoc _ _ _ $@ (_ $@L _) $@ _).
+      + apply cat_binbiprod_pr_eta.
+        * refine ((cat_assoc _ _ _)^$ $@ (_ $@R _) $@ _).
+          1: apply cat_binbiprod_corec_beta_pr1.
+          refine (_ $@ _^$).
+          1: apply cat_binbiprod_pr2_inr.
+          apply cat_binbiprod_pr1_inl.
+        * refine ((cat_assoc _ _ _)^$ $@ (_ $@R _) $@ _).
+          1: apply cat_binbiprod_corec_beta_pr2.
+          refine (_ $@ _^$).
+          1: apply cat_binbiprod_pr1_inr.
+          apply cat_binbiprod_pr2_inl.
+      + apply cat_binbiprod_rec_beta_inl.
+  Defined.
+
+End Symmetry.
+
+(** *** Associativity of binary products *)
+
+Section Associativity.
+
+  Context {A : Type} `{HasBinaryBiproducts A}.
+
+  Local Instance associator_binbiprod
+    : Associator (fun x y => cat_binbiprod x y)
+    := associator_binprod.
+
+  Lemma cate_binbiprod_assoc (x y z : A)
+    : cat_binbiprod x (cat_binbiprod y z)
+      $<~> cat_binbiprod (cat_binbiprod x y) z.
+  Proof.
+    rapply associator_binbiprod.
+  Defined.
+  
+  Definition cat_binbiprod_twist (x y z : A)
+    : cat_binbiprod x (cat_binbiprod y z)
+      $-> cat_binbiprod y (cat_binbiprod x z)
+    := cat_binprod_twist x y z.
+      
+  Lemma cat_binbiprod_twist_inl (x y z : A)
+    : cat_binbiprod_twist x y z $o cat_binbiprod_inl
+      $== cat_binbiprod_inr $o cat_binbiprod_inl.
+  Proof.
+    apply cat_binbiprod_pr_eta.
+    - refine ((cat_assoc _ _ _)^$ $@ (_ $@R _) $@ _).
+      1: apply cat_binbiprod_corec_beta_pr1.
+      refine (cat_assoc _ _ _ $@ _ $@ cat_assoc _ _ _).
+      refine ((_ $@L _) $@ _ $@ (_^$ $@R _)).
+      1: apply cat_binbiprod_pr2_inl.
+      2: apply cat_binbiprod_pr1_inr.
+      refine (_ $@ _^$).
+      1: apply cat_zero_r.
+      apply cat_zero_l.
+    - refine ((cat_assoc _ _ _)^$ $@ (_ $@R _) $@ _).
+      1: apply cat_binbiprod_corec_beta_pr2.
+      refine ((cat_binbiprod_corec_rec _ _ $@R _) $@ _).
+      refine (cat_binbiprod_rec_beta_inl _ _ $@ cat_idr _ $@ _).
+      refine ((cat_idl _)^$ $@ (_^$ $@R _) $@ cat_assoc _ _ _).
+      apply cat_binbiprod_pr2_inr.
+  Defined.
+
+  Lemma cat_binbiprod_twist_inr_inl (x y z : A)
+    : cat_binbiprod_twist x y z $o cat_binbiprod_inr $o cat_binbiprod_inl
+      $== cat_binbiprod_inl.
+  Proof.
+    apply cat_binbiprod_pr_eta.
+    - refine ((cat_assoc _ _ _)^$ $@ (_ $@R _) $@ _).
+      { refine ((cat_assoc _ _ _)^$ $@ (_ $@R _)).
+        1: apply cat_binbiprod_corec_beta_pr1. }
+      refine (cat_assoc _ _ _ $@ _).
+      refine (cat_assoc _ _ _ $@ _).
+      refine ((_ $@L _) $@ _).
+      { refine ((cat_assoc _ _ _)^$ $@ (_ $@R _) $@ _).
+        1: apply cat_binbiprod_pr2_inr. 
+        apply cat_idl. }
+      refine (_ $@ _^$).
+      1,2: apply cat_binbiprod_pr1_inl.
+    - refine ((cat_assoc _ _ _)^$ $@ (_ $@R _) $@ _).
+      { refine ((cat_assoc _ _ _)^$ $@ (_ $@R _)).
+        1: apply cat_binbiprod_corec_beta_pr2. }
+      refine (cat_assoc _ _ _ $@ (_ $@R _) $@ _).
+      1: apply cat_binbiprod_corec_rec.
+      refine ((cat_assoc _ _ _)^$ $@ (_ $@R _) $@ _).
+      1: apply cat_binbiprod_rec_beta_inr.
+      refine (cat_assoc _ _ _ $@ (_ $@L _) $@ _).
+      1: apply cat_binbiprod_pr2_inl.
+      refine (_ $@ _^$).
+      1: apply cat_zero_r.
+      apply cat_binbiprod_pr2_inl.
+  Defined.
+
+  Lemma cat_binbiprod_twist_inr_inr (x y z : A)
+    : cat_binbiprod_twist x y z $o cat_binbiprod_inr $o cat_binbiprod_inr
+      $== cat_binbiprod_inr $o cat_binbiprod_inr.
+  Proof.
+    apply cat_binbiprod_pr_eta.
+    - refine ((cat_assoc _ _ _)^$ $@ (_ $@R _) $@ _).
+      { refine ((cat_assoc _ _ _)^$ $@ (_ $@R _)).
+        1: apply cat_binbiprod_corec_beta_pr1. }
+      refine (cat_assoc _ _ _ $@ _).
+      refine (cat_assoc _ _ _ $@ _).
+      refine ((_ $@L _) $@ _).
+      { refine ((cat_assoc _ _ _)^$ $@ (_ $@R _) $@ _).
+        1: apply cat_binbiprod_pr2_inr. 
+        apply cat_idl. }
+      refine (_ $@ _^$).
+      1: apply cat_binbiprod_pr1_inr.
+      refine ((cat_assoc _ _ _)^$ $@ (_ $@R _) $@ _).
+      1: apply cat_binbiprod_pr1_inr.
+      apply cat_zero_l.
+    - refine ((cat_assoc _ _ _)^$ $@ (_ $@R _) $@ _).
+      { refine ((cat_assoc _ _ _)^$ $@ (_ $@R _)).
+        1: apply cat_binbiprod_corec_beta_pr2. }
+      refine (cat_assoc _ _ _ $@ (_ $@R _) $@ _).
+      1: apply cat_binbiprod_corec_rec.
+      refine ((cat_assoc _ _ _)^$ $@ (_ $@R _) $@ _).
+      1: apply cat_binbiprod_rec_beta_inr.
+      refine (cat_assoc _ _ _ $@ (_ $@L _) $@ _).
+      1: apply cat_binbiprod_pr2_inr.
+      refine (cat_idr _ $@ _^$).
+      refine ((cat_assoc _ _ _)^$ $@ (_ $@R _) $@ _).
+      1: apply cat_binbiprod_pr2_inr.
+      apply cat_idl.
+  Defined.
+
+  Lemma cate_binbiprod_assoc_inl (x y z : A)
+    : cate_binbiprod_assoc x y z $o cat_binbiprod_inl
+      $== cat_binbiprod_inl $o cat_binbiprod_inl.
+  Proof.
+    refine ((_ $@R _) $@ _).
+    1: nrapply Monoidal.associator_twist'_unfold.
+    refine (cat_assoc _ _ _ $@ _).
+    refine ((_ $@L (cat_assoc _ _ _ $@ (_ $@L _))) $@ _).
+    { refine ((cat_binbiprod_corec_rec _ _ $@R _) $@ (_ $@ _)).
+      1: apply cat_binbiprod_rec_beta_inl.
+      apply cat_idr. }
+    simpl.
+    refine ((_ $@L _) $@ _).
+    1: apply cat_binbiprod_twist_inl.
+    refine ((cat_assoc _ _ _)^$ $@ _).
+    refine (_ $@R _).
+    apply cat_binbiprod_swap_inr.
+  Defined.
+
+  Lemma cate_binbiprod_assoc_inr_inl (x y z : A)
+    : cate_binbiprod_assoc x y z $o cat_binbiprod_inr $o cat_binbiprod_inl
+      $== cat_binbiprod_inl $o cat_binbiprod_inr.
+  Proof.
+    refine (((_ $@R _) $@R _) $@ _).
+    1: nrapply Monoidal.associator_twist'_unfold.
+    refine (cat_assoc _ _ _ $@ _).
+    refine (cat_assoc _ _ _ $@ _).
+    refine ((_ $@L (cat_assoc _ _ _ $@ (_ $@L _))) $@ _).
+    { refine ((cat_assoc _ _ _)^$ $@ (_ $@R _)).
+      refine ((cat_binbiprod_corec_rec _ _ $@R _) $@ _).
+      apply cat_binbiprod_rec_beta_inr. }
+    refine ((_ $@L _) $@ _).
+    { refine ((cat_assoc _ _ _)^$ $@ _).
+      refine (((cat_assoc _ _ _)^$ $@R _) $@ _).
+      refine (cat_assoc _ _ _ $@ _).
+      refine ((_ $@L _) $@ _).
+      1: apply cat_binbiprod_swap_inl.
+      apply cat_binbiprod_twist_inr_inr. }
+    refine ((cat_assoc _ _ _)^$ $@ (_ $@R _)).
+    apply cat_binbiprod_swap_inr.
+  Defined.
+  
+  Lemma cate_binbiprod_assoc_inr_inr (x y z : A)
+    : cate_binbiprod_assoc x y z $o cat_binbiprod_inr $o cat_binbiprod_inr
+      $== cat_binbiprod_inr.
+  Proof.
+    refine (((_ $@R _) $@R _) $@ _).
+    1: nrapply Monoidal.associator_twist'_unfold.
+    refine (cat_assoc _ _ _ $@ _).
+    refine (cat_assoc _ _ _ $@ _).
+    refine ((_ $@L (cat_assoc _ _ _ $@ (_ $@L _))) $@ _).
+    { refine ((cat_assoc _ _ _)^$ $@ (_ $@R _)).
+      refine ((cat_binbiprod_corec_rec _ _ $@R _) $@ _).
+      apply cat_binbiprod_rec_beta_inr. }
+    refine ((_ $@L _) $@ _).
+    { refine ((cat_assoc _ _ _)^$ $@ _).
+      refine (((cat_assoc _ _ _)^$ $@R _) $@ _).
+      refine (cat_assoc _ _ _ $@ _).
+      refine ((_ $@L _) $@ _).
+      1: apply cat_binbiprod_swap_inr.
+      apply cat_binbiprod_twist_inr_inl. }
+    apply cat_binbiprod_swap_inl.
+  Defined.
+
+End Associativity.
+
+(** ** Semiadditive Categories *)
+
+Class IsSemiAdditive (A : Type) `{HasEquivs A} := {
+  semiadditive_pointed :: IsPointedCat A;
+  semiadditive_hasbiproducts :: HasBinaryBiproducts A;
+  semiadditive_hasmorext :: HasMorExt A;
+  semiadditive_ishset_hom :: forall (a b : A), IsHSet (a $-> b);
+}.
+
+Section CMonHom.
+
+  Context {A : Type} `{IsSemiAdditive A} (a b : A).
+  
+  (** We can show that the hom-types of a semiadditive category are commutative monoids. *)
+
+  Local Instance zero_hom : Zero (a $-> b) := zero_morphism.
+
+  Local Instance sgop_hom : SgOp (a $-> b) := fun f g =>
+    cat_binbiprod_codiag b
+    $o fmap11 (fun x y => cat_binbiprod x y) f g
+    $o cat_binbiprod_diag a.
+
+  Local Instance left_identity_hom : LeftIdentity sgop_hom zero_hom.
+  Proof.
+    intros g.
+    apply path_hom.
+    unfold sgop_hom, fmap11; cbn.
+    refine (cat_assoc _ _ _ $@ _).
+    refine ((_ $@L cat_assoc _ _ _) $@ _).
+    refine ((cat_assoc _ _ _)^$ $@ _).
+    snrefine ((_ $@L _) $@ _).
+    1: exact cat_binbiprod_inr.
+    { apply cat_binbiprod_pr_eta.
+      - refine (_ $@ cat_binbiprod_pr1_inr^$).
+        refine ((cat_assoc _ _ _)^$ $@ _).
+        refine ((_ $@R _) $@ _).
+        1: apply cat_binbiprod_corec_beta_pr1.
+        refine (cat_assoc _ _ _ $@ _).
+        apply cat_zero_l.
+      - refine (_ $@ cat_binbiprod_pr2_inr^$).
+        refine ((cat_assoc _ _ _)^$ $@ _).
+        refine ((_ $@R _) $@ _).
+        1: apply cat_binbiprod_corec_beta_pr2.
+        refine (cat_assoc _ _ _ $@ _).
+        refine (cat_idl _ $@ _).
+        apply cat_binbiprod_corec_beta_pr2. }
+    nrefine (cat_assoc _ _ _ $@ (_ $@L _) $@ _).
+    { refine ((_ $@R _) $@ _).
+      1: apply cat_binbiprod_corec_rec.
+      apply cat_binbiprod_rec_beta_inr. }
+    refine ((cat_assoc _ _ _)^$ $@ (_ $@R _) $@ _).
+    1: apply cat_binbiprod_rec_beta_inr.
+    apply cat_idl.
+  Defined.
+
+  Local Existing Instance symmetricbraiding_cat_binbiprod.
+
+  (** Using the naturality of swap we can show that the operation is commutative. *)
+  Local Instance commutative_hom : Commutative sgop_hom.
+  Proof.
+    intros f g.
+    apply path_hom.
+    refine (cat_assoc _ _ _ $@ _).
+    refine ((_^$ $@R _) $@ _).
+    1: apply cat_binbiprod_swap_codiag.
+    refine (cat_assoc _ _ _ $@ (_ $@L _) $@ (cat_assoc _ _ _)^$).
+    refine (_ $@ (_ $@L _)).
+    2: apply cat_binbiprod_swap_diag.
+    refine ((cat_assoc _ _ _)^$ $@ (_ $@R _) $@ cat_assoc _ _ _).
+    rapply Monoidal.braid_nat.
+  Defined.
+
+  Local Instance right_identity_ab_hom : RightIdentity sgop_hom zero_hom.
+  Proof.
+    intros f.
+    refine (commutativity _ _ @ _).
+    apply left_identity_hom.
+  Defined.
+
+  Local Instance associative_ab_hom : Associative sgop_hom.
+  Proof.
+    (** There is a lot to unfold here. But drawing out the diagram we can split this into 5 separate diagrams that all commute. Much of the work here will be applying associativity and functor laws to get this diagram in the correct shape. *)
+    intros f g h.
+    apply path_hom.
+    refine (((_ $@L (_ $@R _)) $@R _) $@ _ $@ ((_ $@L (_ $@L _)^$) $@R _)).
+    1,3: refine (fmap_comp _ _ _ $@ (_ $@R _)).
+    1,2: refine (fmap_comp _ _ _ $@ (_ $@L _)).
+    1,2: rapply fmap_comp.
+    do 2 change (fmap (flip (fun x y => cat_binbiprod x y) ?a) ?f)
+      with (fmap10 (fun x y => cat_binbiprod x y) f a);
+    do 2 change (fmap ((fun x y => cat_binbiprod x y) ?b) ?f)
+      with (fmap01 (fun x y => cat_binbiprod x y) b f).
+    Local Notation "a ⊕L g" := (fmap01 (fun x y => cat_binbiprod x y) a g) (at level 99).
+    Local Notation "f ⊕R b" := (fmap10 (fun x y => cat_binbiprod x y) f b) (at level 99).
+    Local Notation "'Δ' x" := (cat_binbiprod_diag x) (at level 10).
+    Local Notation "'∇' x" := (cat_binbiprod_codiag x) (at level 10).
+    change (?w $o ?x $== ?y $o ?z) with (Square z w x y).
+    apply move_right_top.
+    (** The following associativity rewrites are specially chosen so that the diagram can be decomposed easily. *)
+    rapply vconcatL.
+    1: do 2 refine (cat_assoc _ _ _ $@ _).
+    1: refine (((cat_assoc _ _ _)^$ $@R _)).
+    rapply vconcatR.
+    2: do 2 refine ((cat_assoc _ _ _)^$ $@ (_ $@L (cat_assoc _ _ _)) $@ _).
+    2: refine (cat_assoc _ _ _)^$.
+    srapply hconcat.
+    (** We now have to specify the morphism that we are composing along, i.e. the common edge of the two squares where they meet. This is chosen to be the associativity equivalence for biproducts. *)
+    1: nrapply cate_binbiprod_assoc.
+    { nrefine ((_ $@R _) $@ _). 
+      1: rapply Monoidal.associator_twist'_unfold.
+      apply cat_binbiprod_pr_eta.
+      - srefine ((cat_assoc _ _ _)^$ $@ (_ $@R _) $@ _).
+        1: exact (fmap01 (fun x y => cat_binbiprod x y) b cat_binbiprod_pr1).
+        { refine ((cat_assoc _ _ _)^$ $@ (_ $@R _) $@ _).
+          1: apply cat_binbiprod_corec_beta_pr1.
+          refine ((cat_assoc _ _ _)^$ $@ (_ $@R _) $@ _).
+          1: apply cat_binbiprod_corec_beta_pr2.
+          refine (_^$ $@ _). 
+          1: rapply fmap01_comp.
+          refine (fmap02 _ _ _).
+          apply cat_binbiprod_corec_beta_pr2. }
+        refine ((cat_assoc _ _ _)^$ $@ _).
+        refine ((((fmap02 _ _ _ $@ fmap01_id _ _ _)^$ $@ fmap01_comp _ _ _ _)^$ $@R _) $@ _).
+        1: apply cat_binbiprod_corec_beta_pr1.
+        nrefine (cat_idl _ $@ _).
+        refine (_ $@ (_ $@L (cat_assoc _ _ _)^$)).
+        nrefine (_ $@ cat_assoc _ _ _).
+        refine (_ $@ (_^$ $@R _)).
+        2: rapply cat_binbiprod_corec_beta_pr1.
+        refine ((_ $@L _) $@ (cat_assoc _ _ _)^$).
+        nrefine (_ $@ cat_assoc _ _ _).
+        refine (_ $@ (_^$ $@R _)).
+        2: rapply cat_binbiprod_corec_beta_pr1.
+        refine (_ $@ (cat_assoc _ _ _)^$).
+        refine (_ $@ (_ $@L _^$)).
+        2: rapply cat_binbiprod_corec_beta_pr1.
+        symmetry.
+        apply cat_idr.
+      - nrefine ((_ $@L (cat_assoc _ _ _)) $@ _).
+        refine ((cat_assoc _ _ _)^$ $@ _).
+        nrefine ((_ $@R _) $@ _).
+        1: apply cat_binbiprod_corec_beta_pr2.
+        nrefine ((_ $@L (cat_assoc _ _ _)) $@ _).
+        refine ((cat_assoc _ _ _)^$ $@ _).
+        nrefine ((_ $@R _) $@ _).
+        1: apply cat_binbiprod_corec_beta_pr1.
+        nrefine (cat_assoc _ _ _ $@ (_ $@L _) $@ _).
+        { refine ((cat_assoc _ _ _)^$ $@ (_ $@R _)).
+          apply cat_binbiprod_corec_beta_pr2. }
+        nrefine ((_ $@L (cat_assoc _ _ _)) $@ _).
+        refine ((cat_assoc _ _ _)^$ $@ _).
+        nrefine ((_ $@R _) $@ _).
+        1: apply cat_binbiprod_corec_beta_pr1.
+        nrefine ((_ $@L _) $@ _).
+        { refine ((cat_assoc _ _ _)^$ $@ (_ $@R _)).
+          apply cat_binbiprod_corec_beta_pr2. }
+        nrefine ((_ $@L (cat_assoc _ _ _)) $@ _).
+        refine ((cat_assoc _ _ _)^$ $@ _).
+        nrefine ((_ $@R _) $@ _).
+        1: apply cat_binbiprod_corec_beta_pr2.
+        nrefine (cat_idl _ $@ _).
+        refine ((cat_assoc _ _ _)^$ $@ (_ $@R _) $@ _).
+        1: apply cat_binbiprod_corec_beta_pr2.
+        nrefine (cat_assoc _ _ _ $@ _).
+        nrefine (cat_idl _ $@ _).
+        nrefine (cat_binbiprod_corec_beta_pr2 _ _ $@ _).
+        refine (_ $@ (_ $@L (cat_assoc _ _ _)^$)).
+        nrefine (_ $@ cat_assoc _ _ _).
+        refine (_ $@ (_^$ $@R _)).
+        2: apply cat_binbiprod_corec_beta_pr2.
+        refine (_ $@ (cat_assoc _ _ _)^$).
+        refine (_ $@ (cat_idl _)^$).
+        refine (_ $@ (_^$ $@R _) $@ cat_assoc _ _ _).
+        2: apply cat_binbiprod_corec_beta_pr2.
+        refine (_ $@ (cat_assoc _ _ _)^$).
+        refine (_ $@ (cat_idl _)^$).
+        symmetry.
+        apply cat_binbiprod_corec_beta_pr2. }
+    (** We split the square again, this time by picking yet another associativity map as the common edge. This leaves us with a naturality square for associativity. *)
+    srapply hconcat.
+    1: nrapply cate_binbiprod_assoc.
+    1: nrapply Monoidal.associator_nat_m.
+    (** Finally we are left with another polygon which we resolve by brute force. *)
+    refine ((cat_assoc _ _ _)^$ $@ _).
+    apply cat_binbiprod_in_eta.
+    - nrefine (cat_assoc _ _ _ $@ _). 
+      nrefine ((_ $@L _) $@ _).
+      { nrefine ((cat_binbiprod_corec_rec _ _ $@R _) $@ _).
+        apply cat_binbiprod_rec_beta_inl. }
+      refine ((cat_assoc _ _ _)^$ $@ _).
+      refine (cat_idr _ $@ _).
+      refine (cat_assoc _ _ _ $@ (_ $@L _) $@ _).
+      { refine ((cat_binbiprod_corec_rec _ _ $@R _) $@ _).
+        apply cat_binbiprod_rec_beta_inl. }
+      refine ((cat_assoc _ _ _)^$ $@ _).
+      refine (cat_idr _ $@ _).
+      refine (_ $@ _).
+      1: apply cat_binbiprod_rec_beta_inl.
+      symmetry.
+      refine (cat_assoc _ _ _ $@ _).
+      refine ((_ $@L _) $@ _).
+      1: apply cate_binbiprod_assoc_inl.
+      refine ((cat_assoc _ _ _)^$ $@ _).
+      refine ((_ $@R _) $@ _).
+      { refine (cat_assoc _ _ _ $@ (_ $@L _)).
+        refine ((cat_binbiprod_corec_rec _ _ $@R _) $@ _).
+        apply cat_binbiprod_rec_beta_inl. }
+      simpl.
+      refine (cat_assoc _ _ _ $@ _).
+      refine ((_ $@L _) $@ _).
+      { refine (cat_assoc _ _ _ $@ (_ $@L _)).
+        apply cat_binbiprod_rec_beta_inl. }
+      refine ((cat_assoc _ _ _)^$ $@ _).
+      refine ((_ $@R _) $@ _).
+      { refine (cat_assoc _ _ _ $@ (_ $@L _)).
+        refine ((cat_binbiprod_corec_rec _ _ $@R _) $@ (_ $@ _)).
+        1: apply cat_binbiprod_rec_beta_inl.
+        apply cat_idr. }
+      refine (cat_idr _ $@ _).
+      apply cat_binbiprod_rec_beta_inl.
+    - nrefine (cat_assoc _ _ _ $@ _).
+      nrefine ((_ $@L _) $@ _).
+      { nrefine ((cat_binbiprod_corec_rec _ _ $@R _) $@ _).
+        apply cat_binbiprod_rec_beta_inr. }
+      refine ((cat_assoc _ _ _)^$ $@ _).
+      simpl.
+      refine ((_ $@R _) $@ _).
+      { refine (cat_assoc _ _ _ $@ (_ $@L _) $@ _).
+        1: refine ((cat_binbiprod_corec_rec _ _ $@R _) $@ _).
+        1: apply cat_binbiprod_rec_beta_inr.
+        refine ((cat_assoc _ _ _)^$ $@ _).
+        refine ((_ $@R _) $@ _).
+        1: apply cat_binbiprod_rec_beta_inr.
+        apply cat_idl. }
+      simpl.
+      refine (_ $@ (cat_assoc _ _ _)^$).
+      apply cat_binbiprod_in_eta.
+      + refine (cat_assoc _ _ _ $@ _).
+        refine ((_ $@L _) $@ _).
+        { refine ((cat_binbiprod_corec_rec _ _ $@R _) $@ _).
+          apply cat_binbiprod_rec_beta_inl. }
+        refine ((cat_assoc _ _ _)^$ $@ _).
+        refine ((_ $@R _) $@ _).
+        1: apply cat_binbiprod_rec_beta_inl.
+        refine (cat_idr _ $@ _).
+        refine (_ $@ (_ $@L _^$) $@ (cat_assoc _ _ _)^$).
+        2: apply cate_binbiprod_assoc_inr_inl.
+        refine (_ $@ (cat_assoc _ _ _)^$).
+        refine (_ $@ (_ $@L _^$)).
+        2: { refine ((cat_assoc _ _ _)^$ $@ _).
+          refine ((_ $@R _) $@ _).
+          1: refine ((cat_binbiprod_corec_rec _ _ $@R _) $@ _).
+          1: apply cat_binbiprod_rec_beta_inl.
+          simpl.
+          refine (cat_assoc _ _ _ $@ (_ $@L _) $@ _).
+          1: apply cat_binbiprod_rec_beta_inr. 
+          apply cat_idr. }
+        simpl.
+        refine (_ $@ (cat_assoc _ _ _)^$).
+        refine (_^$ $@ (_ $@L _^$)).
+        2: { refine ((cat_binbiprod_corec_rec _ _ $@R _) $@ (_ $@ _)).
+          1: apply cat_binbiprod_rec_beta_inl.
+          apply cat_idr. }
+        apply cat_binbiprod_rec_beta_inl.
+      + refine (cat_assoc _ _ _ $@ _).
+        refine ((_ $@L _) $@ _).
+        { refine ((cat_binbiprod_corec_rec _ _ $@R _) $@ _).
+          apply cat_binbiprod_rec_beta_inr. }
+        refine ((cat_assoc _ _ _)^$ $@ _).
+        refine ((_ $@R _) $@ _).
+        1: apply cat_binbiprod_rec_beta_inr.
+        refine (cat_idl _ $@ _).
+        refine (_ $@ (_ $@L _^$) $@ (cat_assoc _ _ _)^$).
+        2: apply cate_binbiprod_assoc_inr_inr.
+        simpl.
+        refine (_ $@ (cat_assoc _ _ _)^$).
+        refine (_^$ $@ (_ $@L _^$)).
+        2: { refine ((cat_binbiprod_corec_rec _ _ $@R _) $@ (_ $@ _)).
+          1: apply cat_binbiprod_rec_beta_inr.
+          apply cat_idr. }
+        refine (cat_assoc _ _ _ $@ (_ $@L _) $@ _).
+        { refine ((cat_binbiprod_corec_rec _ _ $@R _) $@ _).
+          1: apply cat_binbiprod_rec_beta_inr. }
+        refine ((cat_assoc _ _ _)^$ $@ _).
+        refine ((_ $@R _) $@ _).
+        1: apply cat_binbiprod_rec_beta_inr.
+        apply cat_idl.
+  Defined.
+
+  Local Instance issemigroup_hom : IsSemiGroup (a $-> b) := {}.
+  Local Instance ismonoid_hom : IsMonoid (a $-> b) := {}.
+
+End CMonHom.
+
+(** ** Additive Categories *)
+
+Class IsAdditive (A : Type) `{HasEquivs A} := {
+  additive_semiadditive :: IsSemiAdditive A;
+  additive_negate_hom : forall (a b : A), Negate (a $-> b);
+  additive_left_inverse_hom : forall (a b : A),
+    LeftInverse (sgop_hom a b) (additive_negate_hom a b) (zero_hom a b);
+  additive_right_inverse_hom : forall (a b : A),
+    RightInverse (sgop_hom a b) (additive_negate_hom a b) (zero_hom a b);
+}.
+
+(** Homs in an aditive category form an abelian group. *)
+Definition AbHom {A : Type} `{IsAdditive A} : A -> A -> AbGroup.
+Proof.
+  intros a b.
+  snrapply Build_AbGroup.
+  1: snrapply Build_Group.
+  5: split.
+  - exact (a $-> b).
+  - exact (sgop_hom a b).
+  - exact (zero_hom a b).
+  - exact (additive_negate_hom a b).
+  - exact (ismonoid_hom a b).
+  - exact (additive_left_inverse_hom a b).
+  - exact (additive_right_inverse_hom a b).
+  - exact (commutative_hom a b).
+Defined.
+
+(** TODO: Additive functors *)
